F* can prove false from any well-typedness assumption

examples/unit-tests/stlc.fst
@@ -3,59 +3,148 @@ module Stlc
 open Prims.PURE
 
 type ty =
-  | TyBool  : ty
-  | TyArrow : ty -> ty -> ty
+  | TBool  : ty
+  | TArrow : ty -> ty -> ty
 
-type tm =
-  | TmVar : nat -> tm
-  | TmApp : tm -> tm -> tm
-  | TmAbs : nat -> ty -> tm -> tm
-  | TmTrue : tm
-  | TmFalse : tm
-  | TmIf : tm -> tm -> tm -> tm
+type exp =
+  | EVar   : int -> exp
+  | EApp   : exp -> exp -> exp
+  | EAbs   : int -> ty -> exp -> exp
+  | ETrue  : exp
+  | EFalse : exp
+  | EIf    : exp -> exp -> exp -> exp
 
-val is_value : tm -> Tot bool
-let is_value t =
-  match t with
-  | TmAbs _ _ _ -> true
-  | TmTrue -> true
-  | TmFalse -> true
-  | _ -> false
+val is_value : exp -> Tot bool
+let is_value e =
+  match e with
+  | EAbs _ _ _ -> true
+  | ETrue      -> true
+  | EFalse     -> true
+  | _          -> false
 
 (* Because we only consider call-by-value reduction, we will ever only
    substitute closed values, so this definition of substitution is
    good enough *)
-val subst : nat -> tm -> tm -> Tot tm
-let rec subst x s t =
-  match t with
-  | TmVar xprime ->
-      if x = xprime then s else t
-  | TmAbs xsecond a t1 ->
-      TmAbs xsecond a (if x = xsecond then t1 else (subst x s t1))
-  | TmApp t1 t2 ->
-      TmApp (subst x s t1) (subst x s t2)
-  | TmTrue -> 
-      TmTrue
-  | TmFalse -> 
-      TmFalse
-  | TmIf t1 t2 t3 -> 
-      TmIf (subst x s t1) (subst x s t2) (subst x s t3)
+val subst : int -> exp -> exp -> Tot exp
+let rec subst x e e' =
+  match e' with
+  | EVar xprime -> if x = xprime then e else e'
+(* CH: This fails because F* can't find xsecond for some reason
+  | EAbs xsecond t e1 ->
+      EAbs xsecond t (if x = xsecond then e1 else (subst x e e1))
+*)
+  | EAbs xsecond t e1 -> EAbs xsecond t e1
+  | EApp e1 e2 -> EApp (subst x e e1) (subst x e e2)
+  | ETrue -> ETrue
+  | EFalse -> EFalse
+  | EIf e1 e2 e3 -> EIf (subst x e e1) (subst x e e2) (subst x e e3)
 
+val step : exp -> Tot (option exp)
+let rec step e =
+  match e with
+  | EApp e1 e2 ->
+      if is_value e1 then
+        if is_value e2 then
+          match e1 with
+          | EAbs x t e' -> Some (subst x e2 e')
+          | _           -> None
+        else
+          match (step e2) with
+          | Some e2' -> Some (EApp e1 e2')
+          | None     -> None
+      else begin
+        match (step e1) with
+        | Some e1' -> Some (EApp e1' e2)
+        | None     -> None
+      end
+  | EIf e1 e2 e3 ->
+      if is_value e1 then
+        match e1 with
+        | ETrue   -> Some e2
+        | EFalse  -> Some e3
+        | _       -> None
+      else begin
+        match (step e1) with
+        | Some e1' -> Some (EIf e1' e2 e3)
+        | None     -> None
+      end
+  | _ -> None
 
+type env = int -> Tot (option ty)
 
+val empty : env
+let empty _ = None
 
+(* CH: This should work but it seems that F* stumbles upon the type abbreviation
+val extend : env -> int -> ty -> Tot env
+let extend g x t  = (fun x' -> if x = x' then Some t else g x')
+Expected a term of type "(_:env -> _:int -> _:ty -> Tot env)";
+got a function "(fun g:<UNKNOWN> x:<UNKNOWN> t:<UNKNOWN> x':<UNKNOWN> -> (match (op_Equality x x') with true  -> (Some t)
+	false  -> (g x')))"
+*)
 
+val extend : env -> int -> ty -> int -> Tot (option ty)
+let extend g x t  = (fun x' -> if x = x' then Some t else g x')
 
+let x45 = extend (extend empty 42 TBool) 0 (TArrow TBool TBool)
 
+val extend_eq : g:env -> x:int -> a:ty -> Fact unit
+      (ensures ((extend g x a) x) == Some a)
+let extend_eq g x a = ()
 
+(* CH: turning int into nat we get again the non-trivial precondition problem *)
+val extend_neq : g:env -> x1:int -> a:ty -> x2:int -> Pure unit
+      (requires (x2 =!= x1))
+      (ensures \r => ((extend g x2 a) x1) == g x1)
+let extend_neq g x1 a x2 = ()
 
+(* CH: swapped env and exp args until functions are ignored from the
+   lex ordering or until we can write decreasing clauses *)
+val typing : exp -> env -> Tot (option ty)
+let rec typing e g =
+  match e with
+  | EVar x -> g x
+  | EAbs x t e1 -> begin
+      match typing e1 (extend g x t) with
+      | Some t' -> Some (TArrow t t')
+      | None    -> None
+      end
+  | EApp e1 e2 -> begin
+      match typing e1 g, typing e2 g with
+      | Some (TArrow t11 t12), Some t2 -> if t11 = t2 then Some t12 else None
+      | _                    , _       -> None
+      end
+  | ETrue  -> Some TBool
+  | EFalse -> Some TBool
+  | EIf e1 e2 e3 -> begin
+      (* CH: This triple pattern matching is in fact complete *)
+      match typing e1 g, typing e2 g, typing e3 g with
+      | Some TBool, Some t2, Some t3 -> if t2 = t3 then Some t2 else None
+      | _         , _      , _       -> None
+      end
+  | _ -> None
 
+val canonical_forms_bool : e:exp -> Pure unit
+      (requires ((typing e empty == Some TBool) /\ (is_value e == true)))
+      (ensures \r => (e == true) \/ (e == false))
+let canonical_forms_bool e = ()
 
+val canonical_forms_fun : e:exp -> t1:ty -> t2:ty -> Pure unit
+      (requires ((typing e empty == Some (TArrow t1 t2)) /\ (is_value e == true)))
+      (ensures \r => (exists (x:int). (exists (e':exp). (e == EAbs x t1 e'))))
+let canonical_forms_fun e t1 t2 = ()
 
+(* CH: This is proved without even needing induction or the lemmas,
+   again, too good to be true *)
+val progress : e:exp -> t:ty -> Pure unit
+      (requires (typing e empty == Some t))
+      (ensures \r => (is_value e \/ (exists (e':exp). step e == Some e')))
+let progress e t = ()
 
-
-
-
+val inconsistent : e:exp -> t:ty -> Pure unit
+      (requires (typing e empty == Some t))
+      (ensures \r => False)
+let inconsistent e t = ()
 
 
 
